\begin{equation}
\label{eq:eromodelglobal1}
m\ddot{X} = \xi F_x\cos \theta -\xi F_{sx}\cos \theta + \xi F_{sy} \sin\theta
\end{equation}

\begin{equation}
\label{eq:eromodelglobal2}
m\ddot{Y} = \xi F_x\sin \theta -\xi F_{sx}\sin \theta - \xi F_{sy} \cos \theta
\end{equation}

\begin{equation}
\label{eq:eromodelglobal3}
I\ddot{\theta} = M_{a}+ M_{r},
\end{equation}

\begin{equation*}
\xi = \begin{bmatrix}
1 & 1 & 1 & 1
\end{bmatrix}
\end{equation*}

\begin{equation*}
F_{sx} = \begin{bmatrix}
F_{sxFL} & F_{sxBL} & F_{sxFR} & F_{sxBR}
\end{bmatrix}^T
, \quad
F_{sy} = \begin{bmatrix}
F_{syFL} & F_{syBL} & F_{syFR} & F_{syBR}
\end{bmatrix}^T
\end{equation*}

\begin{equation*}
    F_{sxik}=N_{ik} \mu_{xik} S_{xik}
    ,\quad
    F_{sy}=N_{ik} \mu_{yik} S_{y{ik}}
\end{equation*}

\begin{equation*}
\mu _x = \begin{bmatrix}
\mu _{xFL} & 
\mu _{xBL} & 
\mu _{xFR} & 
\mu _{xBR}
\end{bmatrix}^T
,\quad
\mu _y = \begin{bmatrix}
\mu _{yFL}& 
\mu _{yBL}& 
\mu _{yFR}&
\mu _{yBR}
\end{bmatrix}^T
\end{equation*}

\begin{equation*}
S_x=\begin{bmatrix}
sgn(V_{xFL})&& 
sgn(V_{xBL})&& 
sgn(V_{xFR})&& 
sgn(V_{xBR})
\end{bmatrix}^T
\end{equation*}

\begin{equation*}
S_y=\begin{bmatrix}
sgn(V_{yFL})&& 
sgn(V_{yBL})&& 
sgn(V_{yFR})&& 
sgn(V_{yBR})
\end{bmatrix}^T
\end{equation*}

\begin{equation}
M_r=M_{rx}+M_{ry}
\end{equation}

\begin{equation}
M_{rx}=K^T_xF_{sx},M_{ry}=K^T_yF_{sy}, M_a = K^T_xF_x
\end{equation}

\begin{equation*}
K_x =\begin{bmatrix}
a & a & b & b
\end{bmatrix}^T
,\quad
K_y =\begin{bmatrix}
c & d & c & d
\end{bmatrix}^T
\end{equation*}

\begin{equation*}
F_x= \begin{bmatrix}
F_{FL}&& 
F_{BL}&& 
F_{FR}&& 
F_{BR}
\end{bmatrix}^T
\end{equation*}

\begin{equation*}
    F = \begin{bmatrix}
    F_{FL}+F_{BL} &&
    F_{FR}+F_{BR}
    \end{bmatrix}^T
\end{equation*}

